proved ro soundness for initial program

backend/ValueAnalysis.v
@@ -1187,7 +1187,7 @@ Definition check_add_global (se : Genv.symtbl)
   (b:block)(rm : romem) : romem :=
   match Genv.invert_symbol se b with
   | Some id =>
-      match NMap.get _ b (Genv.find_info se) with
+      match (Genv.find_info se) b with
       | Some (Gvar v) =>
           if v.(gvar_readonly) && negb v.(gvar_volatile) && definitive_initializer v.(gvar_init)
           then PTree.set id (store_init_data_list (ablock_init Pbot) 0 v.(gvar_init)) rm
@@ -1213,7 +1213,7 @@ Proof.
     apply Genv.invert_find_symbol in INV.
     congruence.
   }
-  destruct NMap.get eqn:INFO; eauto.
+  destr.
   destruct g; eauto.
   rewrite PTree.gro; eauto.
   destruct ( gvar_readonly v && negb (gvar_volatile v) && definitive_initializer (gvar_init v)).
@@ -2337,39 +2337,6 @@ Proof.
   - intros. inv H0. inv H. constructor; eauto.
 Qed.
 
-(** ** The initial [ro] soundness for loading process *)
-(** This lemma should be moved to and proved in ValueAnalysis.v.
-       I'm 95% sure it's correct. Maybe we can somehow reuse the initialization
-       proofs in ValueAnalysis for this. Or slightly change the definition of
-       ro_sound_memory using existential [bc] if this approach is more ligheweight. *)
-
-   (** This lemma should also be part of the DR with closed simulation and behavior
-       refinement. We should refer the loading process proposed in CompCertOE *)      
-   Lemma initial_romatch : forall skel m0 se,
-       Genv.init_mem skel = Some m0 ->
-       Genv.symboltbl skel = se ->
-       ValueDomain.romatch (bc_of_symtbl se) m0 (romem_for_symtbl se).
-   Proof.
-     intros. constructor.
-     - unfold romem_for_symtbl in H2.
-       induction (Mem.sup_list (Genv.genv_sup se)); simpl in H2.
-       rewrite Maps.PTree.gempty in H2. congruence.
-       admit. (*ok*)
-     - admit. (*ok *)
-   Admitted.
-
-   Lemma initial_ro_sound :  forall skel m0 se,
-       Genv.init_mem skel = Some m0 ->
-       Genv.symboltbl skel = se ->
-       sound_memory_ro se m0.
-   Proof.
-     intros. constructor. eapply initial_romatch; eauto.
-     apply Genv.init_mem_genv_sup in H as SUP.
-     rewrite <- SUP. rewrite <- H0.
-     apply Mem.sup_include_refl.
-   Qed.
-
-   
 (** ** Block classification for an injection *)
 
 Program Definition bc_of_inj (f: meminj) (se: Genv.symtbl) :=
@@ -2553,12 +2520,7 @@ Proof.
   + eapply bc_of_inj_nostack; eauto.
 Qed.
 
-
-
-
-
-
-
+(*
 (** ** Soundness of the initial memory abstraction *)
 
 Require Import Axioms.
@@ -2694,7 +2656,7 @@ Proof.
   erewrite <- Genv.init_mem_genv_sup in H0 by eauto.
   apply symboltbl_genv_sup in H0 as []. congruence.
 Qed. *)
-
+(*
 Section INIT.
 
 Variable bc: block_classification.
@@ -2958,9 +2920,303 @@ Proof.
   apply inj_of_bc_valid; auto.
   unfold inj_of_bc. erewrite bc_below_invalid; eauto.
 Qed.
-
-
+*)
 End INITIAL.
+*)
+
+(** ** The initial [ro] soundness for loading process *)
+(** 
+    I'm 95% sure it's correct. Maybe we can somehow reuse the initialization
+    proofs in ValueAnalysis for this. Or slightly change the definition of
+    ro_sound_memory using existential [bc] if this approach is more ligheweight. *)
+
+(** This lemma should also be part of the DR with closed simulation and behavior
+    refinement. We could refer the loading process proposed in CompCertOE if necessary *)
+
+
+Lemma romem_valid_exists:
+  forall se id ab,
+    (romem_for_symtbl se) ! id = Some ab ->
+    exists b v,
+      Genv.find_symbol se id = Some b
+      /\ Genv.find_info se b = Some (Gvar v)
+      /\ gvar_readonly v && negb (gvar_volatile v) && definitive_initializer (gvar_init v) = true
+      /\ ab = (store_init_data_list (ablock_init Pbot) 0 (gvar_init v)).
+Proof.
+  intros. unfold romem_for_symtbl in H.
+  induction (Mem.sup_list (Genv.genv_sup se)).
+  - simpl in H. inv H.
+  - simpl in H. unfold check_add_global in H.
+    repeat destr_in H; try rewrite PTree.grspec in H1; destr_in H1.
+    rewrite PTree.gsspec in H0. destr_in H0. inv e.
+    apply Genv.invert_find_symbol in Heqo. exists a, v.
+    splitall; eauto. inv H0. reflexivity.
+Qed.
+
+Lemma store_init_data_summary:
+  forall ab p id,
+  pge Glob (ab_summary ab) ->
+  pge Glob (ab_summary (store_init_data ab p id)).
+Proof.
+  intros.
+  assert (DFL: forall chunk av,
+               vge (Ifptr Glob) av ->
+               pge Glob (ab_summary (ablock_store chunk ab p av))).
+  {
+    intros. simpl. unfold vplub; destruct av; auto.
+    inv H0. apply plub_least; auto.
+    inv H0. apply plub_least; auto.
+  }
+  destruct id; auto.
+  simpl. destruct (propagate_float_constants tt); auto.
+  simpl. destruct (propagate_float_constants tt); auto.
+  apply DFL. constructor. constructor.
+Qed.
+
+Lemma store_init_data_list_summary:
+  forall idl ab p,
+  pge Glob (ab_summary ab) ->
+  pge Glob (ab_summary (store_init_data_list ab p idl)).
+Proof.
+  induction idl; simpl; intros. auto. apply IHidl. apply store_init_data_summary; auto.
+Qed.
+
+Definition ge_match (bc: block_classification) (se : Genv.symtbl) :=
+  forall id b, Genv.find_symbol se id = Some b <-> bc b = BCglob id.
+
+Lemma se_gmatch : forall se,
+    ge_match (bc_of_symtbl se) se.
+Proof.
+  intros. red. unfold bc_of_symtbl; simpl.
+  split; intros.
+  apply Genv.find_invert_symbol in H. rewrite H. reflexivity.
+  destr_in H. inv H. apply Genv.invert_find_symbol. eauto.
+Qed.
+  
+Lemma store_init_data_sound:
+  forall m b p id m' ab bc se
+    (GMATCH : ge_match bc se),
+    Genv.store_init_data se m b p id = Some m' ->
+    bmatch bc m b ab ->
+    bmatch bc m' b (store_init_data ab p id).
+Proof.
+  intros. destruct id; try (eapply ablock_store_sound; eauto; constructor).
+- (* float32 *)
+  simpl. destruct (propagate_float_constants tt); eapply ablock_store_sound; eauto; constructor.
+- (* float64 *)
+  simpl. destruct (propagate_float_constants tt); eapply ablock_store_sound; eauto; constructor.
+- (* space *)
+  simpl in H. inv H. auto.
+- (* addrof *)
+  simpl in H. destruct (Genv.find_symbol _ i) as [b'|] eqn:FS; try discriminate.
+  eapply ablock_store_sound; eauto. constructor. constructor. apply GMATCH. auto.
+Qed.
+
+Lemma store_init_data_list_sound:
+  forall idl m b p m' ab  bc se
+    (GMATCH : ge_match bc se),
+  Genv.store_init_data_list se m b p idl = Some m' ->
+  bmatch bc m b ab ->
+  bmatch bc m' b (store_init_data_list ab p idl).
+Proof.
+  induction idl; simpl; intros.
+- inv H; auto.
+- destruct (Genv.store_init_data _ m b p a) as [m1|] eqn:SI; try discriminate.
+  eapply IHidl; eauto. eapply store_init_data_sound; eauto.
+Qed.
+
+Lemma store_init_data_other:
+  forall m b p id m' ab b' bc se,
+  Genv.store_init_data se m b p id = Some m' ->
+  b' <> b ->
+  bmatch bc m b' ab ->
+  bmatch bc m' b' ab.
+Proof.
+  intros. eapply bmatch_inv; eauto.
+  intros. destruct id; try (eapply Mem.loadbytes_store_other; eauto; fail); simpl in H.
+  inv H; auto.
+  destruct (Genv.find_symbol _ i); try discriminate.
+  eapply Mem.loadbytes_store_other; eauto.
+Qed.
+
+Lemma store_init_data_list_other:
+  forall b b' ab idl m p m'  bc se,
+  Genv.store_init_data_list se m b p idl = Some m' ->
+  b' <> b ->
+  bmatch bc m b' ab ->
+  bmatch bc m' b' ab.
+Proof.
+  induction idl; simpl; intros.
+  inv H; auto.
+  destruct (Genv.store_init_data _ m b p a) as [m1|] eqn:SI; try discriminate.
+  eapply IHidl; eauto. eapply store_init_data_other; eauto.
+Qed.
+
+Lemma store_zeros_same:
+  forall p m b pos n m' bc,
+  store_zeros m b pos n = Some m' ->
+  smatch bc m b p ->
+  smatch bc m' b p.
+Proof.
+  intros until n. functional induction (store_zeros m b pos n); intros.
+- inv H. auto.
+- eapply IHo; eauto. change p with (vplub (I Int.zero) p).
+  eapply smatch_store; eauto. constructor.
+- discriminate.
+Qed.
+
+
+Lemma store_zeros_other:
+  forall b' ab m b p n m' bc,
+  store_zeros m b p n = Some m' ->
+  b' <> b ->
+  bmatch bc m b' ab ->
+  bmatch bc m' b' ab.
+Proof.
+  intros until n. functional induction (store_zeros m b p n); intros.
+- inv H. auto.
+- eapply IHo; eauto. eapply bmatch_inv; eauto.
+  intros. eapply Mem.loadbytes_store_other; eauto.
+- discriminate.
+Qed.
+
+Definition init_bmatch (bc: block_classification) (m: mem) (g: Genv.symtbl) :=
+  forall id b v,
+  Genv.find_symbol g id = Some b -> Genv.find_var_info g b = Some v ->
+  v.(gvar_volatile) = false -> v.(gvar_readonly) = true ->
+  bmatch bc m b (store_init_data_list (ablock_init Pbot) 0 v.(gvar_init)).
+
+Lemma alloc_global_bmatch : forall skel a m g m',
+    let se := Genv.symboltbl skel in
+    Genv.genv_sup g = Mem.support m ->
+    init_bmatch (bc_of_symtbl se) m g ->
+    Genv.alloc_global se m a = Some m' ->
+    init_bmatch (bc_of_symtbl se) m' (Genv.add_global g a).
+Proof.
+  intros. red. intros. assert (GMATCH: ge_match (bc_of_symtbl se) se).
+  apply se_gmatch.
+  unfold Genv.alloc_global in H1. repeat destr_in H1.
+  - (*Gfun*)
+    unfold Genv.find_symbol in H2. simpl in H2.
+    unfold Genv.find_var_info, Genv.find_info in H3. simpl in H3.
+    rewrite PTree.gsspec in H2. destruct (peq id i).
+    inv H2. setoid_rewrite NMap.gss in H3. discriminate.
+    apply Mem.alloc_global_result in Heqp0 as PEQ.
+    unfold Mem.nextblock_global in PEQ. rewrite <- H in PEQ. subst p.
+    assert (Mem.valid_block m b).
+    { red. rewrite <- H. eapply Genv.genv_symb_range; eauto. }
+    assert (b <> (Mem.fresh_block_tid (Genv.genv_sup g) 0)).
+    { apply Mem.valid_not_valid_diff with m; eauto with mem. eapply Mem.fresh_block_alloc_global; eauto. }
+    setoid_rewrite NMap.gso in H3; eauto. repeat destr_in H3.
+    eapply bmatch_inv with m; eauto. eapply H0; eauto.
+    unfold Genv.find_var_info. setoid_rewrite Heqo. reflexivity.
+    intros. transitivity (Mem.loadbytes m0 b ofs n0).
+    eapply Mem.loadbytes_drop; eauto.
+    eapply Mem.loadbytes_alloc_global_unchanged; eauto.
+  - set (sz := init_data_list_size (gvar_init v0)) in *.
+    unfold Genv.find_symbol in H2. simpl in H2.
+    unfold Genv.find_var_info, Genv.find_info in H3. simpl in H3.
+    rewrite PTree.gsspec in H2. destruct (peq id i).
+    + (*new variable block *)
+      subst. inv H2. setoid_rewrite NMap.gss in H3. inv H3.
+      apply Mem.alloc_global_result in Heqp0 as PEQ.
+      unfold Mem.nextblock_global in PEQ. rewrite <- H in PEQ. subst p.
+      apply bmatch_inv with m2. unfold se in Heqo0.
+      eapply store_init_data_list_sound; simpl; eauto.
+      apply ablock_init_sound.
+      eapply store_zeros_same; eauto.
+      split; intros.
+      exploit Mem.load_alloc_global_same; eauto. intros EQ; subst v0; constructor.
+      exploit Mem.loadbytes_alloc_global_same; eauto with coqlib. congruence.
+      intros. eapply Mem.loadbytes_drop; eauto.
+      right; right; right. unfold Genv.perm_globvar. simpl. rewrite H4, H5. constructor.
+    +
+      apply Mem.alloc_global_result in Heqp0 as PEQ.
+      unfold Mem.nextblock_global in PEQ. rewrite <- H in PEQ. subst p.
+      assert (Mem.valid_block m b).
+      { red. rewrite <- H. eapply Genv.genv_symb_range; eauto. }
+      assert (b <> (Mem.fresh_block_tid (Genv.genv_sup g) 0)).
+      { apply Mem.valid_not_valid_diff with m; eauto with mem. eapply Mem.fresh_block_alloc_global; eauto. }
+      setoid_rewrite NMap.gso in H3; eauto. repeat destr_in H3.
+        apply bmatch_inv with m2.
+        eapply store_init_data_list_other; eauto. 
+        eapply store_zeros_other; eauto.
+        apply bmatch_inv with m.
+        eapply H0; eauto. unfold Genv.find_var_info. setoid_rewrite Heqo1. reflexivity.
+        intros. eapply Mem.loadbytes_alloc_global_unchanged; eauto.
+        intros. eapply Mem.loadbytes_drop; eauto.
+Qed.
+
+Lemma alloc_globals_bmatch : forall skel gl m g m',
+    let se := Genv.symboltbl skel in
+    Genv.genv_sup g = Mem.support m ->
+    init_bmatch (bc_of_symtbl se) m g ->
+    Genv.alloc_globals se m gl = Some m' ->
+    init_bmatch (bc_of_symtbl se) m' (Genv.add_globals g gl).
+Proof.
+  induction gl; simpl; intros.
+  - inv H1; auto.
+  - destruct (Genv.alloc_global _ m a) as [m1|] eqn:AG; try discriminate.
+  eapply IHgl; eauto.
+  erewrite Genv.alloc_global_support; eauto. simpl. unfold Mem.nextblock. congruence.
+  eapply alloc_global_bmatch; eauto.
+Qed.
+
+Lemma init_mem_bmatch : forall skel m,
+    let se := Genv.symboltbl skel in
+    Genv.init_mem skel = Some m ->
+    init_bmatch (bc_of_symtbl se) m se.
+Proof.
+  intros.
+  eapply alloc_globals_bmatch; eauto. reflexivity.
+  red. intros. inv H0.
+Qed.
+
+Lemma initial_romatch : forall skel m0 se,
+    Genv.init_mem skel = Some m0 ->
+    Genv.symboltbl skel = se ->
+    romatch (bc_of_symtbl se) m0 (romem_for_symtbl se).
+Proof.
+  intros. constructor.
+  - clear H1.
+    unfold romem_for_symtbl in H2.
+    induction (Mem.sup_list (Genv.genv_sup se)); simpl in H2.
+    rewrite Maps.PTree.gempty in H2. congruence.
+    unfold check_add_global in H2. repeat destr_in H2.
+    + rewrite PTree.grspec in H3. destr_in H3.
+    + rewrite PTree.gsspec in H3. destr_in H3. inv H3.
+      apply store_init_data_list_summary; eauto.
+      simpl. constructor.
+    + rewrite PTree.grspec in H3. destr_in H3.
+    + rewrite PTree.grspec in H3. destr_in H3.
+  - unfold bc_of_symtbl in H1.
+    repeat destr_in H1. destr_in H4. inv H4.
+    apply Genv.invert_find_symbol in Heqo.
+    exploit romem_valid_exists; eauto.
+    intros [b' [v [FIND [INFO [RO ABEQ]]]]]. rewrite FIND in Heqo. inv Heqo.
+    destruct gvar_readonly eqn: READONLY; simpl in RO; try congruence.
+    destruct gvar_volatile eqn: VOLATILE; simpl in RO; try congruence.
+    rename RO into INITIALIZER.
+    exploit Genv.init_mem_characterization; eauto.
+    unfold Genv.find_var_info. rewrite INFO. reflexivity.
+    intros [A [B C]].
+    split.
+    ++ eapply init_mem_bmatch; eauto.
+       unfold Genv.find_var_info. rewrite INFO. reflexivity.
+    ++ intros. intro. apply B in H0. destruct H0 as [E F].
+       unfold Genv.perm_globvar in F. rewrite VOLATILE, READONLY in F. inv F.
+Qed.
+                
+Lemma initial_ro_sound :  forall skel m0 se,
+    Genv.init_mem skel = Some m0 ->
+    Genv.symboltbl skel = se ->
+    sound_memory_ro se m0.
+Proof.
+  intros. constructor. eapply initial_romatch; eauto.
+  apply Genv.init_mem_genv_sup in H as SUP.
+  rewrite <- SUP. rewrite <- H0.
+  apply Mem.sup_include_refl.
+Qed.
 
 Global Hint Resolve areg_sound aregs_sound: va.
 
